Simple lens laws proved with ideal free-var conditions. Also renamed files.

coq/Macro.v
@@ -1,17 +1,17 @@
 Require Import Cases.
-Require Import Term2.
-Require Import Subs2.
-Require Import Match2.
+Require Import Term.
+Require Import Subs.
+Require Import Match.
 Require Import Coq.Classes.RelationClasses.
 Require Import Coq.Setoids.Setoid Coq.Classes.SetoidClass.
 Import StdEnv.
 
 (* TODO: Relax to say (fvar v q -> fvar v p). *)
-Definition same_fvars (p q : term) :=
-  forall v, fvar v p = fvar v q.
+Definition fvars_subset (q p : term) :=
+  forall v, fvar v q = true -> fvar v p = true.
 
 Inductive simple_macro :=
-| smacro (p q : term) : wf p = true -> wf q = true -> same_fvars p q -> simple_macro.
+| smacro (p q : term) : wf p = true -> wf q = true -> fvars_subset q p -> simple_macro.
 
 Fixpoint sexpand m t : option term :=
   match m with
@@ -35,6 +35,96 @@ Fixpoint sunexpand m s t : option term :=
       end
   end.
 
+Definition env_closed a := forall v t,
+  lookup v a = Some t -> closed t.
+
+Lemma mtEnv_closed : env_closed mtEnv.
+Proof.
+  intros. unfold env_closed; intros. discriminate H.
+Qed.
+
+Lemma union_closed : forall a b c,
+  a & b = Some c ->
+  env_closed a ->
+  env_closed b ->
+  env_closed c.
+Proof.
+  unfold env_closed in *; intros a b c C Ha Hb v t L.
+  rewrite lookup_union with (a:=a) (b:=b) in L; try assumption.
+  destruct (mem v a).
+    apply Ha in L; exact L.
+    apply Hb in L; exact L.
+Qed.
+
+Definition closed_tmatch_defn t a := closed t -> env_closed a.
+Lemma closed_tmatch_proof : forall t p a, t / p = Some a -> closed_tmatch_defn t a.
+Proof.
+  apply tmatch_ind; unfold closed_tmatch_defn; intros.
+  Case "q = tvar".
+    unfold env_closed; intros u t L.
+    simpl in L. destruct (VarImpl.beq_var u v); inversion L.
+    rewrite <- H1. exact H.
+  Case "p, q = const n".
+    apply mtEnv_closed.
+  Case "p, q = empty".
+    apply mtEnv_closed.
+  Case "p, q = cons".
+    apply closed_uncons in H4. inversion H4 as (Cp & Cps).
+    apply H1 in Cp. apply H2 in Cps.
+    apply union_closed with (a:=p_q) (b:=ps_qs); assumption.
+Qed.
+Lemma closed_tmatch : forall t p a,
+  t / p = Some a -> closed t -> env_closed a.
+Proof.
+  intros.
+  assert (closed_tmatch_defn t a) by
+    (apply closed_tmatch_proof with (p:=p); assumption).
+  unfold closed_tmatch_defn in H1. auto.
+Qed.
+
+Lemma lookup_compose : forall a b v,
+  lookup v (compose a b) =
+  match lookup v b with
+    | None => lookup v a
+    | Some t => Some (a * t)
+  end.
+Proof.
+  intros.
+  induction b as [ | u t b]; try reflexivity.
+  simpl. destruct (VarImpl.beq_var v u); auto.
+Qed.
+
+Lemma try_lookup__subs : forall v a,
+  try_lookup v a = a * (tvar v).
+Proof. intros. reflexivity. Qed.
+
+Lemma lens_helper : forall t p q t_p a,
+  closed t ->
+  (forall v, fvar v q = true -> fvar v p = true) ->
+  t / p = Some t_p ->
+  t_p * q / q = Some a ->
+  compose t_p a == t_p.
+Proof.
+  intros. intro v.
+  apply lookup_eqv.
+  assert (E: forall v t', lookup v a = Some t' -> lookup v t_p = Some t').
+    intros.
+    apply lookup_subs_tmatch_eq with (ap_p:=a) (p:=q); intros; try assumption.
+    rewrite <- fvar_mem with (p:=t) (q:=p); try assumption.
+    apply H0. exact H4.
+  assert (Ct_p := H1). apply closed_tmatch in Ct_p; auto.
+  assert (Ca: env_closed a).
+    unfold env_closed in *. intros va ta La.
+    apply Ct_p with (v:=va). apply E. exact La.
+  rewrite lookup_compose.
+  destruct (lookup v a) as [t'|] eqn:L.
+  Case "v in a".
+    assert (Ct' := L). apply Ca in Ct'. rewrite closed_subs; try assumption.
+    rewrite E with (t':=t'); try assumption. reflexivity.
+  Case "v not in a".
+    reflexivity.
+Qed.
+
 Lemma simple_lens_1 : forall m t t',
   closed t ->
   sexpand m t = Some t' ->
@@ -45,16 +135,10 @@ Proof.
   simpl in *. destruct (t / p) as [t_p|] eqn:TP; inversion_clear H.
   destruct (t_p * q / q) eqn:TPQ.
   Case "Prove the equivalence".
-    assert (E1: e == t_p).
-      symmetry. apply subs_tmatch_eq with (p:=q).
-      intros. rewrite <- fvar_mem with (p:=t) (q:=p) in H; try assumption.
-      rewrite FV in H. exact H.
-      assumption.
-    assert (E2: t_p * p = t).
-      apply tmatch_subs_eq; assumption.
-    assert (E3: t_p * t = t).
-      apply closed_subs; assumption.
-    rewrite E1. rewrite E2. rewrite E3. reflexivity.
+    rewrite compose_subs_eq.
+    assert (E: compose t_p e == t_p).
+      apply lens_helper with (t:=t) (p:=p) (q:=q); assumption.
+    rewrite E. rewrite tmatch_subs_eq with (p:=t); auto.
   Case "Contradiction : t_p * q / q exists".
     rewrite wf_tmatch_iff in WFq. inversion WFq.
     rewrite H in TPQ. discriminate TPQ.
@@ -115,7 +199,7 @@ Proof.
     SCase "FV condition".
       intros v M. apply mem_compose in M. inversion M.
         erewrite fvar_mem; eauto.
-        rewrite FV. erewrite fvar_mem; eauto.
+        rewrite FV. reflexivity. erewrite fvar_mem; eauto.
   Case "Contradiction : t' / p exists".
     inversion H as [T'].
     rewrite compose_subs_eq in T'.
@@ -123,45 +207,3 @@ Proof.
     apply wf__tmatch with (a := compose s_p t_q) in WFp.
     inversion WFp. rewrite H0 in TP. discriminate TP.
 Qed.
-
-
-
-
-(* Scrap *)
-
-Inductive expand {patt env : Type}
-  {pmatch : Pmatch patt env}
-  {subs : Subs patt env}
-  {lensy : Lensy patt env pmatch subs}
-  (m : @macro patt) (t : patt) (t' : option patt) (n : nat) :=
-| expand_nil : m = mnil -> t' = None -> n = 0 ->
-  expand m t t' n
-| expand_car (p q : patt) (e : env) (m' : macro) :
-  m = mcons p q m' -> pmatch t p = Some e -> t' = Some (subs e q) -> n = 0 ->
-  expand m t t' n
-| expand_cdr (p q : patt) (e : env) (m' : macro) (n' : nat) :
-  m = mcons p q m' -> pmatch t p = None -> expand m' t t' n' -> n = S n' ->
-  expand m t t' n.
-
-Inductive unexpand {patt env : Type}
-  {pmatch : Pmatch patt env}
-  {subs : Subs patt env}
-  {lensy : Lensy patt env pmatch subs}
-  (m : @macro patt) (n : nat) (t : patt) (t' : option patt) :=
-| unexpand_nil : m = mnil -> t' = None ->
-  unexpand m t t'
-| unexpand_car (p q : patt) (e : env) (m' : macro) :
-  m = mcons p q m' -> pmatch t q = Some e -> t' = Some (subs e p) ->
-  unexpand m t t'
-| unexpand_cdr (p q : patt) (e : env) (m' : macro) :
-  m = mcons p q m' -> pmatch t q = None -> unexpand m' t t' ->
-  unexpand m t t'.
-
-Theorem MacroLens : forall (m : macro) (t t' : patt),
-  expand m t (Some t') -> 
-
-Check expand_base.
-
-| expand_rec : m = mcons p q _ -> (
-
-Check foo.
