coq/Term.v
@@ -1,70 +1,30 @@
-Require Import Coq.Bool.Bool.
 Require Import Coq.Arith.EqNat.
-Require Import Coq.Lists.List.
-Require Import Cases.
+Require Import Coq.Bool.Bool.
+
 
 Definition var := nat.
 Definition id := nat.
 Definition beq_var := beq_nat.
 Definition beq_id := beq_nat.
 
-Unset Elimination Schemes.
 Inductive term :=
 | tvar : var -> term
-| node : id -> list term -> term.
-Set Elimination Schemes.
+| const : id -> term
+| empty : term
+| cons : term -> term -> term.
+Notation "p :: q" := (cons p q).
 
-Fixpoint fvar (v : var) (t : term) : bool :=
-  match t with
+
+Fixpoint fvar v p : bool :=
+  match p with
     | tvar v' => beq_var v v'
-    | node _ ts =>
-      (fix fvars (ts : list term) : bool :=
-        match ts with
-          | nil => false
-          | t :: ts => fvar v t || fvars ts
-        end) ts
+    | const c => false
+    | empty => false
+    | p :: ps => fvar v p || fvar v ps
   end.
 
-Definition closed (t : term) : Prop :=
-  forall (v : var), fvar v t = false.
-
-(* Term Induction *)
-
-Definition term_rect := fun
-  (P : term -> Type)
-  (h : forall (v : var), P (tvar v))
-  (g : forall (n : id), P (node n nil))
-  (f : forall (n : id) (t : term) (ts : list term),
-    P t -> P (node n ts) -> P (node n (t :: ts)))
-  =>
-  fix term_rec (t : term) : P t :=
-  match t return P t with
-    | tvar v => h v
-    | node n ts =>
-      ((fix terms_rec (ts : list term) : P (node n ts) :=
-        match ts with
-          | nil => g n
-          | t :: ts => f n t ts (term_rec t) (terms_rec ts)
-        end) ts)
-  end.
-
-Definition term_ind := fun
-  (P : term -> Prop)
-  (h : forall (v : var), P (tvar v))
-  (g : forall (n : id), P (node n nil))
-  (f : forall (n : id) (t : term) (ts : list term),
-    P t -> P (node n ts) -> P (node n (t :: ts)))
-  => term_rect P h g f.
-
-Definition term_rec := fun
-  (P : term -> Set)
-  (h : forall (v : var), P (tvar v))
-  (g : forall (n : id), P (node n nil))
-  (f : forall (n : id) (t : term) (ts : list term),
-    P t -> P (node n ts) -> P (node n (t :: ts)))
-  => term_rect P h g f.
-
-(* Lemmas *)
+Definition closed p : Prop :=
+  forall (v : var), fvar v p = false.
 
 Lemma beq_var_refl : forall (x : var),
   beq_var x x = true.
@@ -73,7 +33,10 @@ Hint Resolve beq_var_refl.
 
 Lemma beq_var_sym : forall (x y : var),
   beq_var x y = beq_var y x.
-Proof. exact NPeano.Nat.eqb_sym. Qed.
+Proof.
+  induction x; induction y; auto.
+  simpl. apply IHx.
+Qed.
 
 Lemma beq_var_trans : forall (x y z : var),
   beq_var x y = true -> beq_var y z = true -> beq_var x z = true.
